Lib/Fin2.v
@@ -3,14 +3,14 @@ Require Export Fin.
 
 Fixpoint fin_lift1 {n} (m : Fin.t n) : Fin.t (S n) := 
     match m with
-    | Fin.F1 n   => @Fin.F1 (S n)
-    | Fin.FS _ m => Fin.FS (fin_lift1 m)
+    | @Fin.F1 n   => @Fin.F1 (S n)
+    |  Fin.FS m => Fin.FS (fin_lift1 m)
     end.
 
 Fixpoint fin_to_nat {n} (m : Fin.t n):= 
     match m with
-    | Fin.F1 _   => 0
-    | Fin.FS _ m => S (fin_to_nat m)
+    | Fin.F1   => 0
+    | Fin.FS m => S (fin_to_nat m)
     end.
 
 Coercion fin_lift1  : Fin.t >-> Fin.t.
