reduction_semantics/reduction_languages_facts.v
@@ -278,7 +278,7 @@ Module Type RED_MINI_LANG2.
   Definition decomp_to_term {k} (d : decomp k) :=
       match d with
       | d_val v   => value_to_term v
-      | d_red _ r c => c[r]
+      | d_red r c => c[r]
       end.
   Coercion decomp_to_term : decomp >-> term.
 
@@ -339,7 +339,7 @@ Module Type RED_MINI_LANG_WD <: RED_MINI_LANG.
   Definition decomp_to_term {k} (d : decomp k) :=
       match d with
       | d_val v   => value_to_term v
-      | d_red _ r c => c[r]
+      | d_red r c => c[r]
       end.
   Coercion decomp_to_term : decomp >-> term.
 
