reduction_semantics/reduction_semantics.v
@@ -149,7 +149,7 @@ Module Type RED_SEM.
   Definition decomp_to_term {k} (d : decomp k) :=
       match d with
       | d_val v   => value_to_term v
-      | d_red _ r c => c[r]
+      | d_red r c => c[r]
       end.
   Coercion decomp_to_term : decomp >-> term.
 
