reduction_semantics/reduction_semantics_facts.v
@@ -1,5 +1,5 @@
-Require Import Util.
-Require Import reduction_languages_facts.
+Require Import Util
+               reduction_languages_facts.
 
 
 
@@ -20,7 +20,7 @@ Module Type DET_RED_MINI_SEM.
   Definition decomp_to_term {k} (d : decomp k) :=
       match d with
       | d_val v   => value_to_term v
-      | d_red _ r c => c[r]
+      | d_red r c => c[r]
       end.
   Coercion decomp_to_term : decomp >-> term.
 
