reduction_semantics/reduction_strategy.v
@@ -53,7 +53,7 @@ Module Type RED_STRATEGY_LANG.
   Coercion decomp_to_term {k} (d : decomp k) :=
       match d with
       | d_val v   => value_to_term v
-      | d_red _ r c => c[r]
+      | d_red r c => c[r]
       end.
 
   Definition dec (t : term) k (d : decomp k) : Prop := 
