refocusing_examples/lam_cl_es_no_tests.v
@@ -1,5 +1,5 @@
-Require Import lam_cl_es_no.
-Require Import abstract_machine_facts.
+Require Import lam_cl_es_no
+               abstract_machine_facts.
 
 
 
