refocusing_examples/lam_no.v
@@ -217,7 +217,7 @@ Module Lam_NO_PreRefSem <: PRE_REF_SEM.
 
 
   Instance dead_is_comp : CompPred ckind dead_ckind.
-      split. destruct x; auto. 
+      split. destruct x; auto.
   Defined.
 
 
@@ -287,7 +287,7 @@ Module Lam_NO_PreRefSem <: PRE_REF_SEM.
   Definition decomp_to_term {k} (d : decomp k) :=
       match d with
       | d_val v     => value_to_term v
-      | d_red _ r c => c[r]
+      | d_red r c => c[r]
       end.
   Coercion decomp_to_term : decomp >-> term.
 
