temp.v
@@ -1,0 +1,3 @@
+Require Import subset.
+
+Check subset.
